DependentComputability/Tactic/NewDPrimStep.lean
@@ -1,0 +1,644 @@
+import DependentComputability.SortExtra
+import Batteries
+namespace DPrimrec.Tactic
+
+open Lean Meta Elab Term Tactic Qq
+
+def projToFn (x : Expr) : MetaM Expr := do
+  if let .proj t i e := x then
+    let info := getStructureInfo (← getEnv) t
+    let some name := info.getProjFn? i |
+      throwError "bad projection: field index {i} out of bounds for type {t}"
+    let type ← inferType e
+    let type ← whnfD type
+    type.withApp fun c args => do
+      unless c.isConstOf t do
+        throwError "bad projection: structure type name mismatch"
+      return .app (mkAppN (.const name c.constLevels!) args) e
+  else
+    return x
+
+inductive ParamComputability where
+  | always
+  | prim
+  | computable
+
+structure TheoremInfo where
+  prim : Bool
+  declName : Name
+  thmName : Name
+  paramInfos : Array ParamComputability
+
+structure DPrimTheorems where
+  primTheorems : NameMap TheoremInfo := {}
+  compTheorems : NameMap TheoremInfo := {}
+deriving Inhabited
+
+def DPrimTheorems.add (ths : DPrimTheorems) (th : TheoremInfo) : DPrimTheorems :=
+  if th.prim then
+    { ths with primTheorems := ths.primTheorems.insert th.declName th }
+  else
+    { ths with compTheorems := ths.compTheorems.insert th.declName th }
+
+initialize dprimExt : SimplePersistentEnvExtension TheoremInfo DPrimTheorems ←
+  registerSimplePersistentEnvExtension {
+    addEntryFn := DPrimTheorems.add
+    addImportedFn xss :=
+      xss.foldl (init := {}) fun acc xs => xs.foldl (init := acc)
+        fun acc x => acc.add x
+  }
+
+def mkThmEntry (thm : Name) : MetaM TheoremInfo := do
+  let val ← getConstVal thm
+  forallTelescope val.type fun xs body => do
+    let mkApp6 (.const thing [clvl, rlvl]) ctx_base ctx α_base α f_base f := body |
+      throwError "invalid `dprim` attribute, conclusion is not DPrimrec or DComputable"
+    let prim ← match thing with
+      | ``DPrimrec => pure true
+      | ``DComputable => pure false
+      | _ => throwError "invalid `dprim` attribute, conclusion is not DPrimrec or DComputable"
+    let .lam nm _ b bi ← whnfR f_base |
+      throwError "invalid `dprim` attribute, conclusion doesn't have a lambda"
+    b.withApp fun x args => do
+      let .const cnm lvls := x |
+        throwError "invalid `dprim` attribute, conclusion must be a const"
+      unless lvls == val.levelParams.tail.map Level.param do
+        throwError "invalid `dprim` attribute, bad level parameters"
+      unless ctx_base == xs[0]! do
+        throwError "expected context parameter {ctx_base} but found {xs[0]!}"
+      unless ctx == xs[1]! do
+        throwError "expected context extra parameter {ctx} but found {xs[1]!}"
+      let mut map : Array ParamComputability := #[]
+      let mut j := 2
+      for h : i in *...args.size do
+        let arg := args[i]
+        if h : j + 1 < xs.size then
+          let var_base := xs[j]
+          unless arg.eta == var_base.app (.bvar 0) do
+            throwError "invalid `dprim` attribute, parameter #{i} is \
+              {Expr.lam nm ctx arg bi} and not {var_base} as expected"
+          if h : j + 2 < xs.size then
+            let x := xs[j + 2]
+            let ty ← inferType x
+            if ty.isAppOf ``DComputable then
+              map := map.push .computable
+              j := j + 3
+            else if ty.isAppOf ``DPrimrec then
+              map := map.push .prim
+              j := j + 3
+            else
+              map := map.push .always
+              j := j + 2
+        else
+          throwError "invalid `dprim` attribute, parameter #{i} out of range"
+      return {
+        prim
+        declName := cnm
+        thmName := thm
+        paramInfos := map
+      }
+
+initialize
+  registerBuiltinAttribute {
+    name := `dprim
+    descr := "Attribute for `dprim_step`"
+    add nm stx kind := do
+      let entry ← MetaM.run' (mkThmEntry nm)
+      modifyEnv (dprimExt.addEntry · entry)
+  }
+
+def finish (e : Expr) (proof : Expr) (goal : MVarId)
+    (vars : Array Expr := #[]) (newGoals : Array MVarId := #[]) : MetaM (Array MVarId) := do
+  match e with
+  | .forallE _ t b bi =>
+    let t := t.instantiateRev vars
+    if bi matches .instImplicit then
+      let inst ← synthInstance t
+      finish b (proof.app inst) goal (vars.push inst) newGoals
+    else
+      let mvar ← mkFreshExprSyntheticOpaqueMVar t
+      finish b (proof.app mvar) goal (vars.push mvar) (newGoals.push mvar.mvarId!)
+  | _ =>
+    goal.assignIfDefEq proof
+    return newGoals
+
+@[match_pattern]
+def mkPSigmaExpr (u v : Level) (nm : Name) (t tt b : Expr) (bi : BinderInfo) : Expr :=
+  mkApp2 (.const ``PSigma [u, v]) t (.lam nm tt b bi)
+
+inductive IsPSigmaExpr : Expr → Nat → Prop where
+  | zero : IsPSigmaExpr e 0
+  | succ {b tt : Expr} {nm : Name} {bi : BinderInfo} (h : IsPSigmaExpr b n) :
+    IsPSigmaExpr (mkPSigmaExpr u v nm t tt b bi) (n + 1)
+
+theorem IsPSigmaExpr.isApp₁ (h : IsPSigmaExpr e n) (hn : n ≠ 0) :
+    e.isApp := by cases h <;> trivial
+theorem IsPSigmaExpr.isApp₂ (h : IsPSigmaExpr e n) (hn : n ≠ 0) :
+    (e.appFn (h.isApp₁ hn)).isApp := by cases h <;> trivial
+theorem IsPSigmaExpr.isConst (h : IsPSigmaExpr e n) (hn : n ≠ 0) :
+    ((e.appFn (h.isApp₁ hn)).appFn (h.isApp₂ hn)).isConst := by cases h <;> trivial
+theorem IsPSigmaExpr.name (h : IsPSigmaExpr e n) (hn : n ≠ 0) :
+    ((e.appFn (h.isApp₁ hn)).appFn (h.isApp₂ hn)).constName! = ``PSigma := by cases h <;> trivial
+theorem IsPSigmaExpr.length (h : IsPSigmaExpr e n) (hn : n ≠ 0) :
+    ((e.appFn (h.isApp₁ hn)).appFn (h.isApp₂ hn)).constLevels!.length = 2 := by cases h <;> trivial
+theorem IsPSigmaExpr.isLambda (h : IsPSigmaExpr e n) (hn : n ≠ 0) :
+    (e.appArg (h.isApp₁ hn)).isLambda := by cases h <;> trivial
+
+@[implemented_by Expr.instantiate1]
+def _root_.Lean.Expr.instantiate1' (e subst : @& Expr) : Expr :=
+  go e subst 0
+where
+  go (e subst : Expr) (depth : Nat) : Expr :=
+    match e with
+    | .bvar n => if n = depth then subst else if n < depth then e else .bvar (n - 1)
+    | .proj nm i e => .proj nm i (go e subst depth)
+    | .mdata d e => .mdata d (go e subst depth)
+    | .lit _ | .const _ _ | .sort _ | .mvar _ | .fvar _ => e
+    | .letE nm t b v nd =>
+      .letE nm (go t subst depth) (go b subst depth) (go v subst (depth + 1)) nd
+    | .forallE nm t b bi => .forallE nm (go t subst depth) (go b subst depth) bi
+    | .lam nm t b bi => .lam nm (go t subst depth) (go b subst (depth + 1)) bi
+    | .app f a => .app (go f subst depth) (go a subst depth)
+
+@[inline]
+def IsPSigmaExpr.getInner (h : IsPSigmaExpr e n) (inst : Expr) (hn : n ≠ 0) : Expr :=
+  have := h.isApp₁ hn
+  have := h.isApp₂ hn
+  let f := e.appFn ‹_› |>.appFn ‹_›
+  let l := e.appArg ‹_›
+  have hf : f.isConst := h.isConst hn
+  have : l.isLambda := h.isLambda hn
+  let .const _ lvls := f
+  let .lam nm t b bi := l
+  b.instantiate1' inst
+
+theorem IsPSigmaExpr.instantiate1'.go (h : IsPSigmaExpr e n) (inst : Expr) (depth : Nat) :
+    IsPSigmaExpr (Expr.instantiate1'.go e inst depth) n := by
+  cases h
+  · constructor
+  · constructor
+    exact go ‹_› inst (depth + 1)
+
+theorem IsPSigmaExpr.instantiate1' (h : IsPSigmaExpr e n) (inst : Expr) :
+    IsPSigmaExpr (e.instantiate1' inst) n := instantiate1'.go h inst 0
+
+theorem IsPSigmaExpr.inner (h : IsPSigmaExpr e n) (inst : Expr) (hn : n ≠ 0) :
+    IsPSigmaExpr (h.getInner inst hn) (n - 1) := by
+  cases h
+  · constructor
+  · apply instantiate1'
+    assumption
+
+@[inline]
+def IsPSigmaExpr.fstExpr (x : Expr) (h : IsPSigmaExpr e n) (hn : n ≠ 0) : Expr :=
+  have := h.isApp₁ hn
+  have := h.isApp₂ hn
+  let f := e.appFn ‹_› |>.appFn ‹_›
+  let l := e.appArg ‹_›
+  have hf : f.isConst := h.isConst hn
+  have : l.isLambda := h.isLambda hn
+  let .const _ lvls := f
+  let .lam nm t b bi := l
+  mkApp3 (.const ``PSigma.fst lvls) t l x
+
+@[inline]
+def IsPSigmaExpr.sndExpr (x : Expr) (h : IsPSigmaExpr e n) (hn : n ≠ 0) : Expr :=
+  have := h.isApp₁ hn
+  have := h.isApp₂ hn
+  let f := e.appFn ‹_› |>.appFn ‹_›
+  let l := e.appArg ‹_›
+  have hf : f.isConst := h.isConst hn
+  have : l.isLambda := h.isLambda hn
+  let .const _ lvls := f
+  let .lam nm t b bi := l
+  mkApp3 (.const ``PSigma.snd lvls) t l x
+
+@[inline]
+def IsPSigmaExpr.mkExpr (x y : Expr) (h : IsPSigmaExpr e n) (hn : n ≠ 0) : Expr :=
+  have := h.isApp₁ hn
+  have := h.isApp₂ hn
+  let f := e.appFn ‹_› |>.appFn ‹_›
+  let l := e.appArg ‹_›
+  have hf : f.isConst := h.isConst hn
+  have : l.isLambda := h.isLambda hn
+  let .const _ lvls := f
+  let .lam nm t b bi := l
+  mkApp4 (.const ``PSigma.mk lvls) t l x y
+
+open Qq in
+partial def mkSigmaType (type : Expr) (n : Nat) (vars : Array Expr := #[]) :
+    MetaM ((u : Level) × { x : Q(Sort u) // IsPSigmaExpr x n } × Expr) := do
+  let cont (nm : Name) (t t' b : Expr) (bi : BinderInfo) :=
+    withLocalDecl nm bi t' fun var => do
+      let l ← getLevel t'
+      match n with
+      | 0 => return ⟨l, ⟨t, .zero⟩, b⟩
+      | k + 1 =>
+        let ⟨u, newT, body⟩ ← mkSigmaType b k (vars.push var)
+        let e := mkPSigmaExpr l u nm t t newT bi
+        return ⟨(levelOne.max l).max u |>.normalize, ⟨e, newT.2.succ⟩, body⟩
+  match type with
+  | .forallE nm t b bi =>
+    let t' := t.instantiateRev vars
+    cont nm t t' b bi
+  | _ =>
+    let .forallE nm t' b bi ← whnf (type.instantiateRev vars) |
+      throwError "invalid type"
+    let t := t'.abstract vars
+    cont nm t t' b bi
+
+partial def mkUncurriedAppArgs (sigma : Expr) (var : Expr) (n : Nat)
+    (hsigma : IsPSigmaExpr sigma n) (args : Array Expr := #[]) : Array Expr :=
+  match n with
+  | 0 => args.push var
+  | k + 1 =>
+    let fst := hsigma.fstExpr var nofun
+    let snd := hsigma.sndExpr var nofun
+    let b := hsigma.getInner fst nofun
+    mkUncurriedAppArgs b snd k (hsigma.inner fst nofun) (args.push fst)
+
+partial def mkUncurriedApp (sigma : Expr) (e var : Expr) (n : Nat)
+    (hsigma : IsPSigmaExpr sigma n) : Expr :=
+  match n with
+  | 0 => .app e var
+  | k + 1 =>
+    let fst := hsigma.fstExpr var nofun
+    let snd := hsigma.sndExpr var nofun
+    let b := hsigma.getInner fst nofun
+    mkUncurriedApp b (.app e fst) snd k (hsigma.inner fst nofun)
+
+partial def mkUncurriedArg (sigma : Expr) (args : Array Expr) (i : Nat := 0)
+    (hi : i < args.size := by grind) (hsigma : IsPSigmaExpr sigma (args.size - i - 1) := by grind) :
+    Expr :=
+  let arg := args[i]
+  if h : i + 1 < args.size then
+    have := by grind
+    let b := hsigma.getInner arg this
+    have _ : IsPSigmaExpr b _ := hsigma.inner arg this
+    let arg2 := mkUncurriedArg b args (i + 1)
+    hsigma.mkExpr arg arg2 this
+  else
+    arg
+
+def idLemma (prim : Bool) : Name :=
+  if prim then ``DPrimrec.id else ``DComputable.id
+
+def constLemma (prim : Bool) : Name :=
+  if prim then ``DPrimrec.const else ``DComputable.const
+
+def proofIrrelLemma (prim : Bool) : Name :=
+  if prim then ``DPrimrec.proof else ``DComputable.proof
+
+def curryLemma (prim : Bool) : Name :=
+  if prim then ``DPrimrec.curry else ``DComputable.curry
+
+def sortLemma (prim : Bool) : Name :=
+  if prim then ``DPrimrec.sort else ``DComputable.sort
+
+def natLitLemma (prim : Bool) : Name :=
+  if prim then `DPrimrec.natLit else `DComputable.natLit
+
+def strLitLemma (prim : Bool) : Name :=
+  if prim then `DPrimrec.strLit else `DComputable.strLit
+
+def predName (prim : Bool) : Name :=
+  if prim then ``DPrimrec else ``DComputable
+
+def mkPred (prim : Bool) {u v : Level}
+    {α_base : Q(Sort u)} {α : Q(convert_to_new_type% $α_base)}
+    {β_base : Q($α_base → Sort v)} {β : Q(convert_to_new_type% $β_base)}
+    {f_base : Q((a : $α_base) → $β_base a)} (f : Q(convert_to_new_type% $f_base)) :
+    Q(Prop) :=
+  if prim then
+    q(DPrimrec $f)
+  else
+    q(DComputable $f)
+
+/-set_option linter.unusedVariables false in
+def constCurryLemma (prim : Bool) (ulvl clvl rlvl : Level) :
+    Q(∀ {β_base : Sort clvl} {β : convert_to_new_type% β_base}
+      {γ_base : β_base → Sort rlvl} {γ : convert_to_new_type% γ_base}
+      {f_base : (a : β_base) → γ_base a} {f : convert_to_new_type% f_base}
+      (hf : DComputable f)
+      {α_base : Sort ulvl} {α : convert_to_new_type% α_base},
+      $(mkPred prim q(convert_to_new% fun _ : α_base => f_base)))= :=
+  match prim with
+  | true => q(@DPrimrec.constCurry.{ulvl, clvl, rlvl})
+  | false => q(@DComputable.constCurry.{ulvl, clvl, rlvl})-/
+
+/-set_option linter.unusedVariables false in
+def compLemma (prim : Bool) (ulvl clvl rlvl : Level) :
+    Q(∀ {β_base : Sort clvl} {β : convert_to_new_type% β_base}
+      {γ_base : β_base → Sort rlvl} {γ : convert_to_new_type% γ_base}
+      {f_base : (a : β_base) → γ_base a} {f : convert_to_new_type% f_base}
+      (hf : DComputable f)
+      {α_base : Sort ulvl} {α : convert_to_new_type% α_base},
+      $(mkPred prim _ _) (convert_to_new% fun _ : α_base => f_base)) :=
+  match prim with
+  | true => q(@DPrimrec.comp.{ulvl, clvl, rlvl})
+  | false => q(@DComputable.comp.{ulvl, clvl, rlvl})-/
+
+partial def whnfFast (e : Expr) (zeta : Bool) (argsRev : Array Expr := #[]) : MetaM Expr := do
+  match e with
+  | .app f a => whnfFast f zeta (argsRev.push a)
+  | .proj .. => return argsRev.foldr (fun a f => f.app a) (← projToFn e)
+  | .mdata _ e => whnfFast e zeta argsRev
+  | .lam .. => if argsRev.isEmpty then return e else whnfFast (e.betaRev argsRev) zeta
+  | .letE _ _ v b _ =>
+    if zeta then
+      whnfFast (b.instantiate1 v) zeta argsRev
+    else
+      return argsRev.foldr (fun a f => f.app a) e
+  | _ => return argsRev.foldr (fun a f => f.app a) e
+
+def matchFunctionType (e : Expr) : MetaM (Level × Expr × Level × Expr) := do
+  let fty ← whnfD e
+  let .forallE nm tt bb bi := fty | throwFunctionExpected e
+  withLocalDeclD `x tt fun x => do
+    let bb' := bb.instantiate1 x
+    return (← getLevel tt, tt, ← getLevel bb', .lam nm tt bb bi)
+
+structure LocalThm where
+  value : Expr
+  paramInfos : Array ParamComputability
+
+def LocalThm.instantiate (thm : LocalThm) (univ : Name) (clvl : Level)
+    (ctx_base ctx : Expr) : Expr :=
+  let repl (lvl : Name) : Option Level := if lvl = univ then clvl else none
+  mkApp2 (thm.value.instantiateLevelParamsCore repl) ctx_base ctx
+
+structure Context where
+  contextUniv : Name
+  localPrimThms : FVarIdMap LocalThm
+  localCompThms : FVarIdMap LocalThm
+  zeta : Bool
+
+abbrev M := ReaderT Context <| ReaderT (FVarIdMap Expr) <| MonadCacheT ExprStructEq Expr MetaM
+
+instance : Inhabited (M α) := ⟨(default : MetaM _)⟩
+
+@[inline]
+def convertToNew (e : Expr) : M Expr := do
+  conversionStepNew.visit e (← readThe _)
+
+@[inline]
+def convertToNewType (ty e : Expr) : M Expr := do
+  return .app (.proj ``SortExtra 0 (← convertToNew ty)) e
+
+@[inline]
+def withNewCtxVar (var_base var : Expr) (act : M α) : M α := do
+  withTheReader (FVarIdMap Expr) (·.insert var_base.fvarId! var) act
+
+@[inline]
+def withBasicLocalThm (prim : Bool) {clvl tlvl : Level}
+    {ctx_base : Q(Sort clvl)} {ctx : Q(convert_to_new_type% $ctx_base)}
+    {res_lam_base : Q($ctx_base → Sort tlvl)} {res_lam : Q(convert_to_new_type% $res_lam_base)}
+    {val_base : Q((a : $ctx_base) → $res_lam_base a)}
+    (val : Q(convert_to_new_type% $val_base))
+    (val_comp : Q($(mkPred prim val)))
+    (act : M α) : M α := do
+  withReader newContext act
+where
+  newContext (c : Context) : Context :=
+    have u := Level.param c.contextUniv
+    match prim with
+    | true =>
+      let value1 := q(@DPrimrec.comp.{u} _ _ _ _ _ _ $val_comp)
+      let value2 := q(@DPrimrec.compComputable.{u} _ _ _ _ _ _ $val_comp)
+      let thm1 : LocalThm := { value := by exact value1, paramInfos := #[.prim] }
+      let thm2 : LocalThm := { value := by exact value2, paramInfos := #[.computable] }
+      { c with localPrimThms := c.localPrimThms.insert val_base.fvarId! thm1,
+               localCompThms := c.localCompThms.insert val_base.fvarId! thm2 }
+    | false =>
+      let value := q(@DComputable.comp.{u} _ _ _ _ _ _ $val_comp)
+      let thm : LocalThm := { value := by exact value, paramInfos := #[.prim] }
+      { c with localCompThms := c.localCompThms.insert val_base.fvarId! thm }
+
+@[inline]
+def isAlwaysZeroQ (lvl : Level) : MaybeLevelDefEq lvl Level.zero :=
+  if lvl.isAlwaysZero then
+    .defEq ⟨⟩
+  else
+    .notDefEq
+
+@[inline]
+def withLetDeclQ [MonadControlT MetaM n] [Monad n]
+    (name : Name) {type : Q(Sort u)} (val : Q($type))
+    (k : (var : Q($type)) → $var =Q $val → n α) : n α :=
+  withLetDecl name type val (fun e => k e ⟨⟩)
+
+@[inline]
+def withHaveDeclQ [MonadControlT MetaM n] [Monad n]
+    (name : Name) {type : Q(Sort u)} (val : Q($type))
+    (k : (var : Q($type)) → n α) : n α :=
+  withLetDecl name type val k (nondep := true)
+
+mutual
+partial def handleUnderApplication (prim : Bool) {clvl rlvl : Level}
+    {ctx_base : Q(Sort clvl)} {ctx : Q(convert_to_new_type% $ctx_base)}
+    {res_base : Q($ctx_base → Sort rlvl)} {res : Q(convert_to_new_type% $res_base)}
+    (f_base : Q((a : $ctx_base) → $res_base a)) (f : Q(convert_to_new_type% $f_base)) :
+    M Q($(mkPred prim f)) := do
+  let .lam nm _ b bi := id f_base | unreachable!
+  let (t', t'lvl, b', b'lvl) ← withLocalDeclQ nm bi q($ctx_base) fun ctx_var => do
+    let ty ← inferType (b.instantiate1 ctx_var)
+    let .forallE nm' t' b' bi' ← whnf ty |
+      throwError "function expected for type {ty} but we have {b.instantiate1 ctx_var}"
+    let t'lvl ← getLevel t'
+    trace[debug] "under-application: {b.instantiate1 ctx_var} has type {ty} : Sort {t'lvl}"
+    let b'lvl ← withLocalDecl nm' bi' t' (getLevel <| b'.instantiate1 ·)
+    pure (Expr.lam nm ctx_base (t'.abstract #[ctx_var]) bi, t'lvl,
+          Expr.lam nm ctx_base
+            (Expr.lam nm' t' (b'.abstract #[ctx_var, .fvar ⟨.anonymous⟩]) bi') bi, b'lvl)
+  have t' : Q($ctx_base → Sort t'lvl) := t'
+  let _newt' : Q(convert_to_new_type% $t') ← convertToNew t'
+  have b' : Q((c : $ctx_base) → $t' c → Sort b'lvl) := b'
+  let _newb' : Q(convert_to_new_type% $b') ← convertToNew b'
+  have : rlvl =QL imax t'lvl b'lvl := ⟨⟩
+  have : $res_base =Q fun c => (x : $t' c) → $b' c x := ⟨⟩
+  have : $res =Q convert_to_new% fun c => (x : $t' c) → $b' c x := ⟨⟩
+  let proof ← solveDPrimGoal false q(fun x : PSigma $t' => $f_base x.1 x.2)
+    q(convert_to_new% fun x : PSigma $t' => $f_base x.1 x.2)
+  match prim with
+  | true => return q(DPrimrec.curry (f := convert_to_new% $f_base) $proof)
+  | false => return q(DComputable.curry (f := convert_to_new% $f_base) $proof)
+
+-- assumes that `f_base` is a lambda
+partial def solveDPrimGoal (prim : Bool) {clvl rlvl : Level}
+    {ctx_base : Q(Sort clvl)} {ctx : Q(convert_to_new_type% $ctx_base)}
+    {res_base : Q($ctx_base → Sort rlvl)} {res : Q(convert_to_new_type% $res_base)}
+    (f_base : Q((a : $ctx_base) → $res_base a)) (f : Q(convert_to_new_type% $f_base)) :
+    M Q($(mkPred prim f)) := withIncRecDepth do
+  withTraceNode `debug (return m!"{exceptEmoji ·} trying to solve goal{indentExpr f}\n\
+    with{indentExpr f_base}") do
+  if let .defEq _ := isAlwaysZeroQ rlvl then
+    match prim with
+    | true => return q((DPrimrec.proof))
+    | false => return q((DComputable.proof))
+  let .lam nm _ b bi := id f_base | unreachable!
+  let b ← whnfFast b (← read).zeta
+  b.withApp fun fn args => do
+  let thm ← match fn with
+    | .sort u =>
+      assert! args.isEmpty
+      return mkApp4 (.const (sortLemma prim) [clvl, u.succ]) ctx_base ctx f_base f
+    | .forallE .. =>
+      assert! args.isEmpty
+      return ← withLocalDecl nm bi ctx_base fun ctx_var => do
+        let univ ← getLevel (fn.instantiate1 ctx_var)
+        return mkApp4 (.const (sortLemma prim) [clvl, univ]) ctx_base ctx f_base f
+    | .lit (.natVal _) =>
+      assert! args.isEmpty
+      return mkApp3 (.const (natLitLemma prim) [clvl]) ctx_base ctx fn
+    | .lit (.strVal _) =>
+      assert! args.isEmpty
+      return mkApp3 (.const (strLitLemma prim) [clvl]) ctx_base ctx fn
+    | .lam .. =>
+      assert! args.isEmpty
+      return ← handleUnderApplication prim q($f_base) q($f)
+    | .letE nm' t v b _ =>
+      let tlvl ← withLocalDecl nm bi ctx_base fun var => getLevel (t.instantiate1 var)
+      have letTy : Q(Sort imax clvl tlvl) := .forallE nm ctx_base t bi
+      let newLetTy : Q(convert_to_new_type% $letTy) ← convertToNew letTy
+      have letVal : Q($letTy) := .lam nm ctx_base v bi
+      let newLetVal : Q(convert_to_new_type% $letVal) ← convertToNew letVal
+      -- add a base variable
+      return ← withLetDeclQ (nm'.appendAfter "_base") q($letVal) fun var_base _ => do
+        -- add a converted variable
+        withLetDeclQ nm' (type := q($newLetTy.1 $letVal)) q($newLetVal)
+          fun (var : Q($newLetTy.1 $letVal)) _ => do
+        withNewCtxVar var_base var do
+          have b := mkAppN (b.instantiate1 (.app var (.bvar 0))) args
+          have f_base' : Q((a : $ctx_base) → $res_base a) := .lam nm ctx_base b bi
+          have : $f_base' =Q $f_base := ⟨⟩
+          let f : Q(convert_to_new_type% $f_base') ← convertToNew f_base'
+          if let .defEq _ := isAlwaysZeroQ tlvl then
+            let res ← solveDPrimGoal prim q($f_base) q($f)
+            return ← mkLetFVars #[var_base, var] res
+          have letTyLam : Q($ctx_base → Sort tlvl) := .lam nm ctx_base t bi
+          let _newLetTyLam : Q(convert_to_new_type% $letTyLam) ← convertToNew letTyLam
+          have : $letTy =Q ∀ c : $ctx_base, $letTyLam c := ⟨⟩
+          have : $newLetTy =Q convert_to_new% ∀ c : $ctx_base, $letTyLam c := ⟨⟩
+          let valcomp ← solveDPrimGoal prim q($letVal) q($newLetVal)
+          have valcomp : Q($(mkPred prim q($var))) := valcomp
+          -- add a computability/primrec proof
+          withHaveDeclQ (nm'.appendAfter "_comp") q($valcomp) fun var_comp => do
+          withBasicLocalThm prim q($var) q($var_comp) do
+            let res ← solveDPrimGoal prim q($f_base') q($f)
+            mkLetFVars #[var_base, var, var_comp] (generalizeNondepLet := false) res
+    | .const nm us =>
+      let state := dprimExt.getState (← getEnv)
+      let thms := if prim then state.primTheorems else state.compTheorems
+      let some thm := thms.get? nm |
+        throwError "no {if prim then "primrec" else "computability"} theorem available for {nm}"
+      pure ⟨.const thm.thmName (.param (← read).contextUniv :: us), thm.paramInfos⟩
+    | .fvar var =>
+      let thms ← if prim then pure (← read).localPrimThms else pure (← read).localCompThms
+      let some thm := thms.get? var |
+        throwError "no local {if prim then "primrec" else "computability"} \
+          theorem available for {fn}"
+      pure thm
+    | .bvar idx =>
+      assert! idx == 0
+      pure ⟨.const (idLemma prim) [.param (← read).contextUniv], #[]⟩
+    | .mvar _ => throwError "expression has metavariables"
+    | .proj .. | .app _ _ | .mdata _ _ => unreachable!
+  if args.isEmpty && thm.paramInfos.isEmpty then
+    -- fast path
+    return thm.instantiate (← read).contextUniv clvl ctx_base ctx
+  if args.size < thm.paramInfos.size then
+    -- under-application
+    return ← handleUnderApplication prim q($f_base) q($f)
+  let mut val := thm.instantiate (← read).contextUniv clvl q($ctx_base) q($ctx)
+  for arg in args, param in thm.paramInfos do
+    let (argT, arglvl) ← withLocalDecl nm bi ctx_base fun var => do
+      let argT ← inferType (arg.instantiate1 var)
+      let arglvl ← getLevel argT
+      return (.lam nm ctx_base argT bi, arglvl)
+    have argT : Q($ctx_base → Sort arglvl) := argT
+    let _newargT : Q(convert_to_new_type% $argT) ← convertToNew argT
+    have argLambda : Q((c : $ctx_base) → $argT c) := .lam nm ctx_base arg bi
+    let newArgLambda : Q(convert_to_new_type% $argLambda) ← convertToNew argLambda
+    val := mkApp2 val argLambda newArgLambda
+    match param with
+    | .always => continue
+    | .prim => panic! "unimplemented"
+    | .computable =>
+      let subgoal ← solveDPrimGoal false q($argLambda) q($newArgLambda)
+      val := .app val subgoal
+  if args.size = thm.paramInfos.size then
+    return val
+  -- over-application (ensure we are in computable territory)
+  let false := prim |
+    withLocalDecl nm bi ctx_base fun var => do
+      throwError "invalid over-application in primrec goal: \
+        expected at most {thm.paramInfos.size} arguments but found {args.size} in\
+        {indentExpr <| b.instantiate1 var}"
+  let type ← withLocalDecl nm bi ctx_base fun var => do
+    let mut type ← inferType (mkAppN fn (args.take thm.paramInfos.size))
+    if type.getForallArity < args.size - thm.paramInfos.size then
+      type ← liftM <| forallBoundedTelescope type (some (args.size - thm.paramInfos.size))
+          mkForallFVars
+    return type.abstract #[var]
+  let mut newType ← convertToNew type
+  trace[debug] "handling over-application ({thm.paramInfos.size} < {args.size}):\
+    {indentExpr f}\nwith{indentExpr newType}"
+  let mut b := mkAppN fn (args.take thm.paramInfos.size)
+  let mut newB ←
+    withLocalDeclQ nm bi q($ctx_base) fun var_base => do
+    withLocalDeclQ nm bi q($ctx.1 $var_base) fun var => do
+    withNewCtxVar var_base var do
+      let res ← convertToNew (b.instantiate1 var_base)
+      return res.abstract #[var_base, var]
+  for arg in args[thm.paramInfos.size...*] do
+    let mkApp4 (.const ``New.Forall [t'lvl, b'lvl]) t'_base t' b'_base b' := id newType |
+      --withLocalDecl nm bi ctx_base fun var => do
+        --throwFunctionExpected ((mkAppN b args).instantiate1 var)
+        let newType2 := Expr.lam (nm.appendAfter "_base") ctx_base
+          (.lam nm (mkExtraApp ctx (.bvar 0)) newType bi) bi
+        throwError "function expected but we have{indentExpr newType2}"
+    have t'lam : Q($ctx_base → Sort t'lvl) := .lam nm ctx_base t'_base bi
+    have b'lam : Q((c : $ctx_base) → $t'lam c → Sort b'lvl) := .lam nm ctx_base b'_base bi
+    have bLambda : Q((c : $ctx_base) → (a : $t'lam c) → $b'lam c a) := .lam nm ctx_base b bi
+    have argLambda : Q((c : $ctx_base) → $t'lam c) := .lam nm ctx_base arg bi
+    have _newt'lam : Q(convert_to_new_type% $t'lam) :=
+      .lam (nm.appendAfter "_base") ctx_base (.lam nm (mkExtraApp ctx (.bvar 0)) t' bi) bi
+    have _newb'lam : Q(convert_to_new_type% $b'lam) :=
+      .lam (nm.appendAfter "_base") ctx_base (.lam nm (mkExtraApp ctx (.bvar 0)) b' bi) bi
+    have newBLambda : Q(convert_to_new_type% $bLambda) :=
+      .lam (nm.appendAfter "_base") ctx_base (.lam nm (mkExtraApp ctx (.bvar 0)) newB bi) bi
+    let newArgLambda : Q(convert_to_new_type% $argLambda) ← convertToNew argLambda
+    have val' : Q(DComputable (convert_to_new% $bLambda)) := val
+    let argProof ← solveDPrimGoal false q($argLambda) q($newArgLambda)
+    val := q(DComputable.app $val' $argProof)
+    newType := b'.beta #[arg, newArgLambda.bindingBody!.bindingBody!]
+    b := b.app arg
+    newB := mkApp2 newB arg newArgLambda.bindingBody!.bindingBody!
+  return val
+
+end
+
+elab "dcomp_tac" : tactic => do
+  let goal ← getMainGoal
+  goal.withContext do
+  let type ← withReducible <| goal.getType'
+  let mkApp6 (.const ``DComputable [clvl, rlvl]) ctx_base ctx res_base res f_base f := type |
+    throwError "invalid goal for dcomp_tac: {type}"
+  have ctx_base : Q(Sort clvl) := ctx_base
+  have _ctx : Q(convert_to_new_type% $ctx_base) := ctx
+  have res_base : Q($ctx_base → Sort rlvl) := res_base
+  have _res : Q(convert_to_new_type% $res_base) := res
+  have f_base : Q((c : $ctx_base) → $res_base c) := f_base
+  have f : Q(convert_to_new_type% $f_base) := f
+  let ctxUniv := mkFreshLevelName (← getLevelNames)
+  let context := {
+    contextUniv := ctxUniv
+    localPrimThms := {}
+    localCompThms := {}
+    zeta := false
+  }
+  let baseMap ← populateBaseMap
+  let res ← (solveDPrimGoal false q($f_base) q($f)).run context |>.run baseMap |>.run
+  goal.assign res
+
+end DPrimrec.Tactic
